Update sortByScore.dfy

proj/proj_verify/sortByScore.dfy
@@ -1,34 +1,62 @@
-// Use insertion sort algorithm
+// Insertion sort
+// Sorts the blood score - descending order
 
-predicate Sorted(a: array<int>, low:int, high:int)
- requires a != null // 1.9.7
- requires 0<=low<=high<=a.Length
- reads a
- { forall j,k:: low<=j<k<high ==> a[j]<=a[k] }
- 
- 
-method InsertionSortSwap(a: array<int>)
-requires a != null // 1.9.7
-requires a.Length > 1
-ensures Sorted(a, 0, a.Length);
-ensures multiset(a[..]) == multiset(old(a[..]));
-modifies a;
+
+class Blood {
+	var score :real;
+  
+	constructor(s :real)
+		modifies this
+		ensures score == s
+	{
+		score := s;
+	}
+}
+
+
+predicate Sorted(a: seq<Blood>, low:int, high:int)
+	//requires a != null
+	requires 0<=low<=high<=|a|//.Length
+	reads a
 {
- var up:=1;
- while (up < a.Length)
- invariant 1 <= up <= a.Length;
- invariant Sorted(a, 0, up);
- invariant multiset(a[..]) == multiset(old(a[..]));
- {
- var down := up; // the next unordered element
- while (down >= 1 && a[down-1] > a[down])
- invariant 0 <= down <= up;
- invariant forall i,j:: (0<=i<j<=up && j!=down) ==> a[i]<=a[j];
- invariant multiset(a[..]) == multiset(old(a[..]));
- {
- a[down-1], a[down] := a[down], a[down-1];
- down:=down-1;
- }
- up:=up+1;
- }
+	forall j,k:: low<=j<k<high ==> a[j].score>=a[k].score
+}
+ 
+ 
+//bList - List of wanted blood
+
+method sortByScore(bList: array<Blood>) returns (sorted :seq<Blood>)
+	requires bList != null
+	requires bList.Length > 1
+	ensures Sorted(bList[..], 0, |bList[..]|)
+  ensures multiset(old(bList)[..]) == multiset(sorted)
+  ensures multiset(bList[..]) == multiset(sorted)
+	modifies bList
+{
+	var i:=1;
+
+  var u :seq<Blood> := bList[..];
+  assert u == old(bList)[..];
+  assert u == bList[..];
+  assert multiset(u) == multiset(u);
+  assert multiset(bList[..]) == multiset(u);
+  assert multiset(u) == multiset(old(bList)[..]);
+  
+	while (i < bList.Length)
+		invariant 1 <= i <= bList.Length;
+		invariant Sorted(bList[..], 0, i);
+		invariant multiset(bList[..]) == multiset(u);
+	{
+		var j := i;
+		while (j >= 1 && bList[j-1].score < bList[j].score)
+			invariant 0 <= j <= i;
+			invariant forall x,y:: (0<=x<y<=i && y!=j) ==> bList[x].score>=bList[y].score;
+			invariant multiset(bList[..]) == multiset(u);
+		{
+			bList[j-1], bList[j] := bList[j], bList[j-1];
+			j:=j-1;
+		}
+		i:=i+1;
+	}
+  sorted := bList[..];
 }
